EffectSSA/ProofSketch/VarSet.lean
@@ -65,6 +65,9 @@ instance : EmptyCollection VarSet where emptyCollection := empty
 def singleton (v : VarId) : VarSet := ofSet { v }
 instance : Singleton VarId VarSet where singleton := singleton
 
+def insert (v : VarId) (V : VarSet) : VarSet := ofSet (Set.insert v V.toSet)
+instance : Insert VarId VarSet where insert := insert
+
 def Mem (A : VarSet) (v : VarId) := v ∈ A.toSet
 instance : Membership VarId VarSet where mem := Mem
 
@@ -88,6 +91,11 @@ theorem ext (h : ∀ x, x ∈ A ↔ x ∈ B) : A = B := by
   show A.toSet = B.toSet
   ext x
   simpa using h x
+
+/-! ### mem -/
+
+@[simp, grind =] theorem mem_singleton : x ∈ ({ y } : VarSet) ↔ x = y := by rfl
+@[simp, grind =] theorem mem_insert : x ∈ (Insert.insert y A) ↔ x = y ∨ x ∈ A := by rfl
 
 /-! ### empty -/
 section Empty
@@ -174,6 +182,9 @@ attribute [local grind] Disjoint
 @[simp, grind .] theorem empty_disjoint : Disjoint ∅ A := by grind
 @[simp, grind .] theorem disjoint_empty : Disjoint A ∅ := by grind
 @[simp, grind =] theorem disjoint_self : A.Disjoint A ↔ A = ∅ := by grind
+
+@[simp, grind =] theorem singleton_disjoint_iff : ({ x } : VarSet).Disjoint A ↔ x ∉ A := by
+  simp [Disjoint, eq_empty_iff]
 
 @[simp, grind =] theorem union_disjoint :
     Disjoint (A ∪ B) C ↔ Disjoint A C ∧ Disjoint B C := by
