EffectSSA/ProofSketch/CaseStudy/ConstFold.lean
@@ -1,0 +1,421 @@
+module
+
+public import EffectSSA.ProofSketch.ProofSketch
+public import EffectSSA.ProofSketch.Rewrite
+public import EffectSSA.ProofSketch.InstArr
+public import EffectSSA.ProofSketch.Tactic
+
+namespace EffectSSA.ProofSketch
+public section
+
+namespace CaseStudy.ConstFold
+
+inductive SimpleArith
+  /-- `$n` -/
+  | const (n : Nat)
+  | add
+  deriving DecidableEq
+
+instance : SSA SimpleArith Unit Nat where
+  initialState := ()
+  instDenote := {
+    denote i _ xs := ((), match i, xs with
+      | .const n, [] => [n]
+      | .add, [x, y] => [x + y]
+      | _, _ => []
+    )
+  }
+
+/-- `$x := $n` -/
+abbrev constOp (x : VarId) (n : Nat) : Inst SimpleArith where
+  results := [x]
+  opCode := .const n
+  args := []
+
+/-- `$x := add($y, $z)` -/
+abbrev addOp (x y z : VarId) : Inst SimpleArith where
+  results := [x]
+  opCode := .add
+  args := [y, z]
+
+@[simp] theorem results_constOp : (constOp x n).results = [x] := by rfl
+@[simp] theorem args_constOp : (constOp x n).args = [] := by rfl
+
+@[simp] theorem resultsSet_constOp : (constOp x n).resultsSet = {x} := by
+  ext; simp
+@[simp] theorem argsSet_constOp : (constOp x n).argsSet = ∅ := by
+  ext; simp
+
+@[simp] theorem results_addOp : (addOp x y z).results = [x] := by rfl
+@[simp] theorem args_addOp : (addOp x y z).args = [y, z] := by rfl
+
+@[simp] theorem resultsSet_addOp : (addOp x y z).resultsSet = {x} := by
+  ext; simp
+@[simp] theorem argsSet_addOp : (addOp x y z).argsSet = {y, z} := by
+  ext; simp
+
+/-! ## Semantics Simplification -/
+
+@[simp, grind =] theorem denote_constOp :
+    ⟦constOp x c⟧ ρ = { ρ with locals := ρ.locals.with x c } := by
+  simp [(⟦·⟧)]
+
+@[simp, grind =] theorem denote_addOp :
+    ⟦addOp x y z⟧ ρ = (SEnv.getD <| do
+      let y ← ρ.locals y
+      let z ← ρ.locals z
+      return { ρ with locals := ρ.locals.with x (y + z) }) := by
+  simp only [Denote.denote, List.mapM_cons, List.mapM_nil, Option.pure_def, Option.bind_eq_bind,
+    Option.bind_some]
+  cases ρ.locals y; simp
+  cases ρ.locals z <;> simp
+
+/-! ## WellBehavedness -/
+
+/--
+All instructions of `SimpleArith` are pure, and thus well-behaved.
+-/
+@[simp, grind .]
+axiom wellbehaved (i : Inst SimpleArith) : i.HasEqn
+
+/-! ## Rewrite Family & Soundness -/
+
+/-- `$x := $c₁; $y := $c₂; $z := add($x, $y)` ⟹ `...; $z := ${c₁ + c₂}` -/
+@[expose] def constFoldRw (x y z : VarId) (c₁ c₂ : Nat) : Rewrite SimpleArith 3 where
+  src := .ofVector #v[
+    [constOp x c₁],
+    [constOp y c₂],
+    [addOp z x y]
+  ]
+  tgt := .ofVector #v[
+    [constOp x c₁],
+    [constOp y c₂],
+    [constOp z (c₁ + c₂)],
+  ]
+  wellbehaved_src := by grind
+  wellbehaved_tgt := by grind
+
+/-- `$x := $c₁; $z := add($x, $x)` ⟹ `...; $z := ${c₁ + c₁}` -/
+@[expose] def constFoldRwAlt (x z : VarId) (c₁ : Nat) : Rewrite SimpleArith 2 where
+  src := .ofVector #v[
+    [constOp x c₁],
+    [addOp z x x]
+  ]
+  tgt := .ofVector #v[
+    [constOp x c₁],
+    [constOp z (c₁ + c₁)],
+  ]
+  wellbehaved_src := by grind
+  wellbehaved_tgt := by grind
+
+/-!
+`constFoldRwAlt` seems a bit duplicated, it is really just a specialization of `constFoldRw`.
+The need for it arises from our definition of "completeness" of a context, which currently
+states that a context must contain *all* holes.
+
+In our case, if we have a rewrite like `constFoldRw x y y c c`, then the first
+and second hole are identical, thus this rewrite would be perfectly safe to
+apply in a context which does not mention (at most) one of the first or second
+hole. In fact, if we wanted to apply this rewrite in a real program, then both
+"hole"s really just refer to the exact same instruction, and thus only one of
+the hole *can* even be mentionened.
+
+Thus `constFoldRwAlt` exists, which has just the one constant.
+
+Ideally, though, we would like to say that for that particular instance of the
+3-ary rewrite `constFoldRw`, the notion of completeness is a bit more relaxed
+to be able to use that one as-is.
+-/
+
+@[simp, grind .]
+theorem constFoldRw.isSound : (constFoldRw x y z c₁ c₂).IsSound := by
+  simp only [Rewrite.IsSound, Pattern.DenRefine, Pattern.getElem_hole]
+  rintro ⟨_|_|_⟩ ρ η hρη
+  · suffices ⟦constOp x c₁⟧ ρ ⊒ ⟦constOp x c₁⟧ η by
+      rintro - -; simpa [constFoldRw]
+    grind
+  · suffices ⟦constOp y c₂⟧ ρ ⊒ ⟦constOp y c₂⟧ η by
+      rintro - -; simpa [constFoldRw]
+    grind
+  · rintro h -
+    have ⟨hx, hy⟩ : ρ.locals x = some c₁ ∧ ρ.locals y = some c₂ := by
+      replace h :
+          let S := (constFoldRw x y z c₁ c₂).src
+          S.EqnLemma x ρ ∧ S.EqnLemma y ρ := by
+        simp [constFoldRw, Pattern.EqnLemmaUpTo] at h
+        grind [constFoldRw]
+      simp only [Pattern.EqnLemma] at h
+      have := h.1 [constOp x c₁] (by simp [constFoldRw])
+      have := h.2 [constOp y c₂] (by simp [constFoldRw])
+      grind [Inst.EqnLemma]
+    suffices ⟦addOp z x y⟧ ρ ⊒ ⟦constOp z (c₁ + c₂)⟧ η by simpa [constFoldRw]
+    grind
+
+@[simp, grind .]
+theorem constFoldRwAlt.isSound : (constFoldRwAlt x z c₁).IsSound := by
+  simp only [Rewrite.IsSound, Pattern.DenRefine, Pattern.getElem_hole]
+  rintro ⟨_|_⟩ ρ η hρη
+  · suffices ⟦constOp x c₁⟧ ρ ⊒ ⟦constOp x c₁⟧ η by
+      rintro - -; simpa [constFoldRw]
+    grind
+  · rintro h -
+    have hx : ρ.locals x = some c₁ := by
+      replace h : (constFoldRwAlt x z c₁).src.EqnLemma x ρ := by
+        simp [constFoldRwAlt, Pattern.EqnLemmaUpTo] at h
+        grind [constFoldRwAlt]
+      simp only [Pattern.EqnLemma] at h
+      specialize h [constOp x c₁] (by simp [constFoldRwAlt])
+      grind [Inst.EqnLemma]
+    suffices ⟦addOp z x x⟧ ρ ⊒ ⟦constOp z (c₁ + c₁)⟧ η by simpa [constFoldRwAlt]
+    grind
+
+/-! ## Implementation -/
+
+abbrev Program := InstArr SimpleArith
+
+/-! ### Matchers -/
+
+/--
+`is.matchConst x` returns `some n` if the instruction that defines
+variable `x` in `is` is a constant with value `n` (i.e, `constOp x n`).
+-/
+def Program.matchConst (is : Program) (x : VarId) : Option Nat :=
+  go is.toSeq
+where go : List (Inst SimpleArith) → Option Nat
+  | [] => none
+  | { opCode := .const n, args := [], results := [x'] } :: is =>
+      if x = x' then some n else go is
+  | _ :: is => go is
+
+/-- `matchAdd i` returns `some (x, y, z)` if `i` is a (well-formed) addition
+instruction, with `x` as the resulting variable and arguments `y` and `z`.
+That is, if `i` is equal to `addOp x y z`. -/
+def matchAdd : Inst SimpleArith → Option (VarId × VarId × VarId)
+  | { opCode := .add, args := [y, z], results := [x] } => some (x, y, z)
+  | _ => none
+
+@[simp, grind =] theorem matchAdd_eq_some_iff :
+    matchAdd i = some r ↔ i = addOp r.1 r.2.1 r.2.2 := by
+  simp [matchAdd, addOp]; grind
+
+open Program in
+@[grind →]
+theorem constOp_mem_of_matchConst_eq_some {acc : Program} :
+    acc.matchConst x = some c → constOp x c ∈ acc.toSeq := by
+  rcases acc with ⟨⟨is⟩⟩
+  simp only [matchConst, InstArr.toSeq]
+  fun_induction matchConst.go x is <;> grind
+
+/-! ### ConstFold -/
+
+/--
+`constFold is` returns an equivalent program, after a constant-folding pass.
+-/
+@[expose]
+def constFold (is : Program) : Program :=
+  go (.emptyWithCapacity is.size) is.toSubarray
+where
+  /--
+  `foldInst? acc i` attempts to constant fold instruction `i` (referring to
+  `acc` for the instructions that define `i`'s arguments), or returns `none`
+  if `i` is not a well-formed, constant-foldable `add` instruction.
+  -/
+  foldInst? (acc : Program) (i : Inst SimpleArith) : Option (Inst SimpleArith) :=
+    do
+    let (x, y, z) ← matchAdd i
+    let c₁ ← acc.matchConst y
+    let c₂ ← acc.matchConst z
+    return constOp x (c₁ + c₂)
+  /--
+  `foldInst acc i` attempts to constant fold instruction `i` with `foldInst?`,
+  returning the original instruction unchanged if constant folding failed
+  for any reason.
+  -/
+  foldInst acc i := (foldInst? acc i).getD i
+  go (acc : Program) (is : InstSubarray SimpleArith) : Program :=
+    if _ : is.size = 0 then
+      acc
+    else
+      let i := foldInst acc is[0]
+      go (acc.push i) is.popFront
+  termination_by is.size
+
+section FoldInstLemmas
+variable {acc : Program} {i : Inst SimpleArith}
+
+@[simp, grind =]
+theorem constFold.foldInst?_eq_some_iff :
+    foldInst? acc i = some i' ↔ ∃ x y z,
+      i = addOp x y z
+      ∧ ∃ c₁, acc.matchConst y = some c₁
+      ∧ ∃ c₂, acc.matchConst z = some c₂
+      ∧ i' = constOp x (c₁ + c₂) := by
+  simp [foldInst?, Option.bind_eq_some_iff]; grind
+
+@[simp] theorem constFold.argsSet_foldInst : (foldInst acc i).argsSet ⊆ i.argsSet := by
+  unfold foldInst; cases hi : foldInst? acc i <;> grind
+grind_pattern constFold.argsSet_foldInst => (constFold.foldInst acc i).argsSet
+
+@[simp, grind .] theorem constFold.results_foldInst : (foldInst acc i).results = i.results := by
+  unfold foldInst; cases hi : foldInst? acc i <;> grind
+@[simp, grind .] theorem constFold.resultsSet_foldInst : (foldInst acc i).resultsSet = i.resultsSet := by
+  simp [Inst.resultsSet]
+
+@[grind ←]
+theorem constFold.wellFormed_foldInst :
+    (acc.push i).toSeq.WellFormed ∅ → (acc.push <| foldInst acc i).toSeq.WellFormed ∅ := by
+  grind
+
+/--
+Prove that a single step of the constant folder is sound.
+
+This proof is still somewhat long, but it is *purely syntactical*.
+Any semantic reasoning has already been done in
+`Rewrite.isRefinedBy_of_contextual_isRefinedBy` and
+in the proofs that the rewrites are (locally) sound.
+-/
+theorem constFold.foldInst_sound (wf : (acc.push i).toSeq.WellFormed ∅) :
+    ⟦acc.push i⟧ {} ⊒ ⟦acc.push <| foldInst acc i⟧ {} := by
+  have wf' : (acc.push <| foldInst acc i).toSeq.WellFormed ∅ := by grind
+  unfold foldInst at *
+  cases hi? : foldInst? acc i
+  case none =>
+    -- There was no match, thus `foldInst` was a no-op
+    grind
+  case some i' =>
+    -- There *was* a match, so now we show that there is a context `C` and
+    -- rewrite `rw` s.t. `(acc.push i).toSeq` is `C[rw.srw]` and
+    -- `(acc.push i').toSeq` is `C[rw.tgt]`
+    obtain ⟨x, y, z, hi, c₁, hy, c₂, hz, hi'⟩ : ∃ x y z,
+          i = addOp x y z
+          ∧ ∃ c₁, acc.matchConst y = some c₁
+          ∧ ∃ c₂, acc.matchConst z = some c₂
+          ∧ i' = constOp x (c₁ + c₂) := by
+        simpa using hi?
+    have wf' := by simpa only [hi?, Option.getD_some] using wf'
+    simp only [Option.getD_some]
+
+    -- We know that `x` cannot be the same variable as `y` nor `z`
+    have : x ≠ y ∧ x ≠ z := by
+      have hy : (addOp x y z).resultsSet.Disjoint (constOp y c₁).resultsSet := by grind
+      have hz : (addOp x y z).resultsSet.Disjoint (constOp z c₂).resultsSet := by grind
+      exact ⟨by simpa using hy, by simpa using hz⟩
+
+    -- Consider whether the two arguments to the addition are the same or not,
+    -- to determine which rewrite to instantiate, and how to construct the
+    -- context to use as witness
+    by_cases hyz : y = z
+    case' pos =>
+      obtain ⟨rfl, rfl⟩ : y = z ∧ c₁ = c₂ := by grind
+      -- Since y = z, use the alternate rewrite, with a single constant
+      let rw := constFoldRwAlt y x c₁
+      -- Invoke the core theory's main result
+      apply rw.isRefinedBy_of_contextual_isRefinedBy
+      · exact constFoldRwAlt.isSound
+      · grind
+      · assumption
+
+      -- The witness context:
+      exists (acc.push i).toSeq.toContext [[y], [x]]
+      and_intros
+      · simp only [reduceCompleteToContext]
+        and_intros; grind
+        · exists constOp y c₁; grind
+        · exists i; grind
+      · rw [InstSeq.plug_toContext_eq_self_of]
+        intro j hj idx hidx hres
+        match idx with
+        | 0 | 1 =>
+          simpa using (by apply InstSeq.eq_of_results_eq _ hj <;> grind)
+        | _+2 => contradiction
+
+      · suffices (InstSeq.toContext [[y], [x]] acc.toSeq).plug rw.tgt = acc.toSeq by
+          have toHole_i : i.toHole [[y], [x]] = .inr ⟨1, by grind⟩ := by
+            rw [Inst.toHole_eq_inr_iff, hi]
+            simp [List.idxOf?_eq_some_iff]
+            grind
+          simp [this, toHole_i, hi']
+        rw [InstSeq.plug_toContext_eq_self_of]
+        intro j hj idx hidx hres
+        match idx with
+        | 0 =>
+          simpa using (by apply InstSeq.eq_of_results_eq _ hj <;> grind)
+        | 1 =>
+          exfalso
+          have hjr : j.results = [x] := by grind
+          have : i.resultsSet.Disjoint j.resultsSet := by grind
+          simp [Inst.resultsSet, hjr, hi, VarSet.eq_empty_iff] at this
+        | _+2 => contradiction
+
+
+    case' neg =>
+      -- Since y ≠ z, use the full rewrite
+      let rw := constFoldRw y z x c₁ c₂
+      -- Invoke the core theory's main result
+      apply rw.isRefinedBy_of_contextual_isRefinedBy
+      · exact constFoldRw.isSound
+      · grind
+      · assumption
+      -- The witness context:
+      exists (acc.push i).toSeq.toContext [[y], [z], [x]]
+      and_intros
+      · simp only [reduceCompleteToContext]
+        refine ⟨by grind, ?_⟩
+        and_intros
+        · exists constOp y c₁; grind
+        · exists constOp z c₂; grind
+        · exists i; grind
+
+      · rw [InstSeq.plug_toContext_eq_self_of]
+        intro j hj idx hidx hres
+        match idx with
+        | 0 | 1 | 2 =>
+          simpa using (by
+            apply InstSeq.eq_of_results_eq _ hj
+            <;> simp -failIfUnchanged <;> grind)
+        | _+3 => contradiction
+
+      · suffices (InstSeq.toContext [[y], [z], [x]] acc.toSeq).plug rw.tgt = acc.toSeq by
+          have toHole_i : i.toHole [[y], [z], [x]] = .inr ⟨2, by grind⟩ := by
+            simp only [Inst.toHole_eq_inr_iff]; grind
+          simp [this, toHole_i, hi']
+        rw [InstSeq.plug_toContext_eq_self_of]
+        intro j hj idx hidx hres
+        match idx with
+        | 0 | 1 =>
+          simpa using (by apply InstSeq.eq_of_results_eq _ hj <;> grind)
+        | 2 =>
+          exfalso
+          have hjr : j.results = [x] := by grind
+          have : i.resultsSet.Disjoint j.resultsSet := by grind
+          simp [Inst.resultsSet, hjr, hi, VarSet.eq_empty_iff] at this
+        | _+3 => contradiction
+
+end FoldInstLemmas
+
+/--
+Prove that the constant folder is sound.
+This is just a straightforward induction around `constFold.foldInst_sound`.
+-/
+theorem constFold_sound {is : Program}
+    (wf : is.toSeq.WellFormed ∅) :
+    ⟦is⟧ {} ⊒ ⟦constFold is⟧ {} := by
+  let is := is.toSubarray
+  suffices ∀ acc, (acc.toSeq ++ is.toSeq).WellFormed ∅ →
+      ⟦acc.toSeq ++ is.toSeq⟧ {} ⊒ ⟦constFold.go acc is⟧ {} by
+    specialize this .empty (by grind); simpa [is]
+  clear wf
+  intro acc
+  fun_induction constFold.go acc is
+  case case1 => grind
+  case case2 acc is hsize i' ih =>
+    intro wf
+    suffices ⟦acc.toSeq ++ is.toSeq⟧ { } ⊒ ⟦(acc.push i').toSeq ++ is.popFront.toSeq⟧ { } by
+      apply Refinement.trans this <| ih ?_
+      grind
+    suffices ⟦acc.push is[0]⟧ { } ⊒ ⟦acc.push i'⟧ { } by
+      grind
+    apply constFold.foldInst_sound
+    · grind
+
+#print axioms constFold_sound
